Fix DSP proofs

new/proof/github_com/goose_lang/goose/testdata/examples/channel.v
@@ -910,8 +910,8 @@ Instance mapper_service_prot_unfold Φpre Φpost :
     (mapper_service_prot_aux Φpre Φpost (mapper_service_prot Φpre Φpost)).
 Proof. apply proto_unfold_eq, (fixpoint_unfold _). Qed.
 
-Definition is_mapper_stream γ stream : iProp Σ :=
-  ∃ req_ch res_ch f (Φpre : go_string → iProp Σ) (Φpost : go_string → go_string → iProp Σ),
+Definition is_mapper_stream stream : iProp Σ :=
+  ∃ γ req_ch res_ch f (Φpre : go_string → iProp Σ) (Φpost : go_string → go_string → iProp Σ),
   ⌜stream = {| stream.req' := req_ch; stream.res' := res_ch; stream.f' := f |}⌝ ∗
   "Hf_spec" ∷ □ (∀ (s: go_string),
       Φpre s → WP #f #s {{ λ v, ∃ (s': go_string), ⌜v = #s'⌝ ∗ Φpost s s' }}) ∗
@@ -923,7 +923,7 @@ Lemma wp_mkStream (f: func.t) Φpre Φpost :
                         Φpre strng -∗ WP #f #strng {{ λ v, ∃ (s': go_string), ⌜v = #s'⌝ ∗ Φpost strng s' }}) }}}
     @! chan_spec_raw_examples.mkStream #f
   {{{ γ stream, RET #stream;
-      is_mapper_stream γ stream ∗
+      is_mapper_stream stream ∗
     # (stream.(stream.req'), stream.(stream.res')) ↣{γ} mapper_service_prot Φpre Φpost }}}.
 Proof.
   wp_start. wp_auto.
@@ -941,12 +941,11 @@ Proof.
     [by eauto|by eauto|..].
   iModIntro. wp_auto.
   iApply "HΦ".
+  simpl. iSplitR "Hpl"; [ | iFrame ]. (* iSplit is for performance *)
   rewrite /is_mapper_stream /=.
-  iSplitR "Hpl".
-  { iExists _, _, _, _, _. iSplit; [done|].
-    iDestruct "Hpre" as "#Hpre". iFrame "Hpr".
-    iIntros "!>" (s) "HΦ". by iApply "Hpre". }
-  iFrame "Hpl".
+  iExists _, _, _, _, _, _. iSplit; [done|].
+  iDestruct "Hpre" as "#Hpre". iFrame "Hpr".
+  iIntros "!>" (s) "HΦ". by iApply "Hpre".
 Qed.
 
 Lemma wp_MapServer (my_stream: stream.t) :
@@ -961,7 +960,7 @@ Proof using chan_protocolG0 chan_protocolG1 globalsGS0.
   iAssert (
     "s" ∷ s_ptr ↦ my_stream ∗
 
-    "Hprot" ∷ # (my_stream.(stream.res'), my_stream.(stream.req')) ↣
+    "Hprot" ∷ # (my_stream.(stream.res'), my_stream.(stream.req')) ↣{γ}
                  iProto_dual (mapper_service_prot Φpre Φpost)
   )%I with "[s Hf_spec Hprot]" as "IH".
   { iFrame. subst. iFrame. }
@@ -999,14 +998,14 @@ Proof using chan_protocolG0 chan_protocolG1 contributionG0 H dspG0 globalsGS0.
     {
        iIntros (s) "!> _". wp_auto. by eauto.
     }
-    iIntros (stream).
+    iIntros (γ stream).
     iIntros "Hmapper".
     wp_auto.
     wp_apply (wp_mkStream _ (λ _, True)%I (λ s1 s2, ⌜s2 = s1 ++ "!"%go⌝)%I).
     {
        iIntros (s) "!> _". wp_auto. by eauto.
     }
-    iIntros (s').
+    iIntros (γ' s').
     iIntros "H'".
     wp_auto.
     iDestruct "Hmapper" as "[Hmapper Hstr]".
@@ -1091,11 +1090,11 @@ Proof using chan_protocolG0 chan_protocolG1 contributionG0 H dspG0 globalsGS0.
   { wp_apply (wp_Muxer with "[Hcons]"); [|done]. iFrame "Hmpmc Hcons". }
   wp_apply (wp_mkStream _ (λ _, True)%I (λ s1 s2, ⌜s2 = s1 ++ ","%go⌝)%I).
   { iIntros (s) "!> _". wp_auto. by eauto. }
-  iIntros (stream1) "[Hstream1 Hc1]".
+  iIntros (γ1 stream1) "[Hstream1 Hc1]".
   wp_auto.
   wp_apply (wp_mkStream _ (λ _, True)%I (λ s1 s2, ⌜s2 = s1 ++ "!"%go⌝)%I).
   { iIntros (s) "!> _". wp_auto. by eauto. }
-  iIntros (stream2) "[Hstream2 Hc2]".
+  iIntros (γ2 stream2) "[Hstream2 Hc2]".
   wp_auto.
   wp_apply (wp_mpmc_send with "[$Hmpmc $Hprod $Hstream1]").
   iIntros "Hprod".
